LAS/LAA preserved undefined/final/initial states. DAE preserved final states.
git-svn-id: https://webdav.seas.upenn.edu/svn/sol/vol@3879 eef5ea85-cc2e-0410-bd84-0fae1f012da8

src3.0/Transforms/laa.v
@@ -431,9 +431,9 @@ Definition cmds_simulation (pinfo: PhiInfo) (laainfo: LAAInfo pinfo) (f1:fdef)
 
 Definition block_simulation (pinfo: PhiInfo) (laainfo: LAAInfo pinfo) f1 b1 b2
   : Prop :=
-  if (fdef_dec (PI_f pinfo) f1) then
-    subst_block (LAA_lid pinfo laainfo) [! pinfo !] b1 = b2
-  else b1 = b2.
+  (if (fdef_dec (PI_f pinfo) f1) then
+    subst_block (LAA_lid pinfo laainfo) [! pinfo !] b1
+  else b1) = b2.
 
 Lemma fdef_simulation__eq_fheader: forall pinfo laainfo f1 f2
   (H: fdef_simulation pinfo laainfo f1 f2),
@@ -533,9 +533,9 @@ Qed.
 
 Definition cmd_simulation (pinfo: PhiInfo) (laainfo: LAAInfo pinfo) (f1:fdef)
   c c': Prop :=
-if (fdef_dec (PI_f pinfo) f1) then
-  subst_cmd (LAA_lid pinfo laainfo) [! pinfo !] c = c'
-else c = c'.
+(if (fdef_dec (PI_f pinfo) f1) then
+  subst_cmd (LAA_lid pinfo laainfo) [! pinfo !] c
+else c) = c'.
 
 (* same to las' *)
 Lemma cmds_simulation_cons_inv: forall pinfo laainfo F c1 cs2 cs',
@@ -875,13 +875,30 @@ Qed.
 (* same to las' *)
 Definition pars_simulation (pinfo: PhiInfo) (laainfo: LAAInfo pinfo) (f1:fdef)
   (ps1 ps2:params) : Prop :=
-  if (fdef_dec (PI_f pinfo) f1) then
+  (if (fdef_dec (PI_f pinfo) f1) then
     (List.map
       (fun p =>
        let '(t, v):=p in
        (t, subst_value (LAA_lid pinfo laainfo) [! pinfo !] v)) ps1)
-    = ps2
-  else ps1 = ps2.
+  else ps1) = ps2.
+
+(* same to las' *)
+Lemma getEntryBlock__simulation: forall pinfo laainfo f1 f2 b2,
+  getEntryBlock f2 = Some b2 ->
+  fdef_simulation pinfo laainfo f1 f2 ->
+  exists b1, getEntryBlock f1 = Some b1 /\ 
+    block_simulation pinfo laainfo f1 b1 b2.
+Proof.
+  unfold fdef_simulation.
+  unfold block_simulation.
+  intros.
+  destruct (fdef_dec (PI_f pinfo) f1); inv H0; eauto.
+    remember (PI_f pinfo) as R1.
+    destruct R1 as [[? ? ? a ?] b]; simpl in *.
+    destruct b; simpl in *; inv H.
+    exists b. 
+    split; auto.
+Qed.
 
 (* same to las' *)
 Lemma fdef_simulation__entry_block_simulation: forall pinfo laainfo F1 F2 B1 B2,
@@ -889,7 +906,12 @@ Lemma fdef_simulation__entry_block_simulation: forall pinfo laainfo F1 F2 B1 B2,
   getEntryBlock F1 = ret B1 ->
   getEntryBlock F2 = ret B2 ->
   block_simulation pinfo laainfo F1 B1 B2.
-Admitted. (* fsim *)
+Proof.
+  intros.
+  eapply getEntryBlock__simulation in H1; eauto.
+  destruct H1 as [b1 [J1 J2]].
+  uniq_result. auto.
+Qed.
 
 (* same to las' *)
 Lemma fdef_simulation_inv: forall pinfo laainfo fh1 fh2 bs1 bs2,
@@ -911,10 +933,10 @@ Qed.
 (* same to las' *)
 Definition par_simulation (pinfo: PhiInfo) (laainfo: LAAInfo pinfo) (f1:fdef)
   (p p':typ * attributes * value) : Prop :=
-if (fdef_dec (PI_f pinfo) f1) then
+(if (fdef_dec (PI_f pinfo) f1) then
   let '(t, v) := p in
-  (t, v {[ [! pinfo !] // LAA_lid pinfo laainfo]}) = p'
-else p = p'.
+  (t, v {[ [! pinfo !] // LAA_lid pinfo laainfo]})
+else p) = p'.
 
 (* same to las' *)
 Lemma pars_simulation_cons_inv: forall pinfo laainfo F p1 ps2 ps',
@@ -1690,34 +1712,458 @@ Lemma find_st_ld__laainfo: forall l0 ps0 cs0 tmn0 v cs (pinfo:PhiInfo) dones
     LAA_block pinfo laainfo = (block_intro l0 ps0 cs0 tmn0).
 Admitted. (* laainfo *)
 
+(* same to las *)
 Lemma s_genInitState__laa_State_simulation: forall pinfo laainfo S1 S2 main
-  VarArgs cfg2 IS2,
-  system_simulation pinfo laainfo S1 S2 ->
-  Opsem.s_genInitState S2 main VarArgs Mem.empty = ret (cfg2, IS2) ->
+  VarArgs cfg2 IS2
+  (Hssim: system_simulation pinfo laainfo S1 S2)
+  (Hinit: Opsem.s_genInitState S2 main VarArgs Mem.empty = ret (cfg2, IS2)),
   exists cfg1, exists IS1,
     Opsem.s_genInitState S1 main VarArgs Mem.empty = ret (cfg1, IS1) /\
     State_simulation pinfo laainfo cfg1 IS1 cfg2 IS2.
-Admitted. (* laainfo *)
+Proof.
+  unfold Opsem.s_genInitState.
+  intros.
+  inv_mbind'.
+  destruct m as [los nts ps].
+  inv_mbind'.
+  destruct b as [l0 ps0 cs0 tmn0].
+  destruct f as [[fa rt fid la va] bs].
+  inv_mbind'. symmetry_ctx.
+  assert (HlkF2FromS2:=HeqR).
+  eapply TopSim.system_simulation__fdef_simulation_r2l in HeqR; eauto.
+  destruct HeqR as [f1 [HlkF1fromS1 Hfsim]]. simpl in Hfsim.
+  fill_ctxhole.
+  eapply TopSim.system_simulation__getParentOfFdefFromSystem in HeqR0; eauto.
+  destruct HeqR0 as [m1 [J1 J2]].
+  fill_ctxhole. destruct m1 as [los1 nts1 ps1].
+  destruct J2 as [J2 [J3 J4]]; subst.
+  eapply TopSim.genGlobalAndInitMem_spec in HeqR1; eauto.
+  destruct HeqR1 as [gl1 [fs1 [M1 [HeqR1 [EQ1 [EQ2 EQ3]]]]]]; subst.
+  fill_ctxhole.
+  assert (J:=HeqR2).
+  eapply getEntryBlock__simulation in J; eauto.
+  destruct J as [b1 [J5 J6]].
+  fill_ctxhole.
+  destruct b1 as [l2 ps2 cs2 tmn2].
+  destruct f1 as [[fa1 rt1 fid1 la1 va1] bs1].
+  assert (J:=Hfsim).
+  apply fdef_simulation__eq_fheader in J.
+  inv J.
+  fill_ctxhole.
+  match goal with
+  | |- exists _:_, exists _:_, Some (?A, ?B) = _ /\ _ => exists A; exists B
+  end.
+  match goal with 
+  | H: getParentOfFdefFromSystem _ _ = _ |- _ =>
+    apply getParentOfFdefFromSystem__moduleInProductsInSystemB in H;
+    destruct H as [HMinS HinPs]
+  end.
+  assert (J:=J6).
+  apply block_simulation_inv in J.
+  destruct J as [J1 [J2 [J3 J7]]]; subst.
+  assert (blockInFdefB (block_intro l0 ps0 cs0 tmn0)
+           (fdef_intro (fheader_intro fa rt fid la va) bs) = true) as HBinF.
+    apply entryBlockInFdef; auto.
+  repeat (split; auto).
+    exists l0. exists ps2. exists nil. auto.
+    exists l0. exists ps0. exists nil. auto.
+Qed.
 
+(* same to las *)
+Lemma cmds_simulation_nil_inv' : forall (pinfo : PhiInfo) 
+  (laainfo : LAAInfo pinfo) (f1 : fdef) (cs : list cmd),
+  cmds_simulation pinfo laainfo f1 cs nil -> cs = nil.
+Proof.
+  unfold cmds_simulation. intros.
+  destruct_if; auto.
+    destruct cs; inv H1; auto.
+Qed.
+
+(* same to las *)
+Lemma cmds_simulation_cons_inv' : forall (pinfo : PhiInfo) 
+  (laainfo : LAAInfo pinfo) (f1 : fdef) (cs : list cmd) c2 cs2,
+  cmds_simulation pinfo laainfo f1 cs (c2::cs2) -> 
+  exists c1, exists cs1, 
+    cs = c1::cs1 /\
+    cmd_simulation pinfo laainfo f1 c1 c2 /\
+    cmds_simulation pinfo laainfo f1 cs1 cs2.
+Proof.
+  unfold cmds_simulation, cmd_simulation. intros.
+  destruct_if; eauto.
+    destruct cs; inv H1; eauto.
+Qed.
+
+(* same to las *)
+Inductive tmn_simulation' (pinfo:PhiInfo) (laainfo:LAAInfo pinfo) (F:fdef) 
+  : terminator -> terminator -> Prop :=
+| tmn_simulation_return : forall id0 t0 v v',
+    value_simulation pinfo laainfo F v v' ->
+    tmn_simulation' pinfo laainfo F (insn_return id0 t0 v) (insn_return id0 t0 v')
+| tmn_simulation_return_void : forall id0,
+    tmn_simulation' pinfo laainfo F (insn_return_void id0) (insn_return_void id0)
+| tmn_simulation_br : forall id0 v v' l1 l2,
+    value_simulation pinfo laainfo F v v' ->
+    tmn_simulation' pinfo laainfo F (insn_br id0 v l1 l2) (insn_br id0 v' l1 l2)
+| tmn_simulation_br_uncond : forall id0 l0,
+    tmn_simulation' pinfo laainfo F (insn_br_uncond id0 l0) 
+                                    (insn_br_uncond id0 l0)
+| tmn_simulation_unreachable : forall id0,
+    tmn_simulation' pinfo laainfo F (insn_unreachable id0) 
+                                    (insn_unreachable id0)
+.
+
+(* same to las *)
+Lemma tmn_simulation'__refl: forall pinfo laainfo F t,
+  PI_f pinfo <> F ->
+  tmn_simulation' pinfo laainfo F t t.
+Proof.
+  intros.
+  destruct t; constructor; auto using value_simulation__refl.
+Qed.
+
+(* same to las *)
+Lemma tmn_simulation__tmn_simulation': forall pinfo laainfo F t t'
+  (Htsim: tmn_simulation pinfo laainfo F t t'),
+  tmn_simulation' pinfo laainfo F t t'.
+Proof.
+  unfold tmn_simulation.
+  intros.
+  destruct (fdef_dec (PI_f pinfo) F); subst; auto using tmn_simulation'__refl.
+    destruct t; simpl;
+    constructor; try solve [
+      unfold value_simulation;
+      destruct (fdef_dec (PI_f pinfo) (PI_f pinfo)); try congruence; auto
+    ].
+Qed.
+
+(* same to las *)
+Ltac inTmnOp_isnt_stuck v H3 Hwfcfg1 Hwfpp1 :=
+match type of Hwfpp1 with
+| OpsemPP.wf_State 
+              {|
+              OpsemAux.CurSystem := _;
+              OpsemAux.CurTargetData := ?td;
+              OpsemAux.CurProducts := _;
+              OpsemAux.Globals := ?gl;
+              OpsemAux.FunTable := _ |}
+    {| Opsem.ECS := {| Opsem.CurFunction := _;
+                       Opsem.CurBB := ?b;
+                       Opsem.CurCmds := nil;
+                       Opsem.Terminator := ?tmn;
+                       Opsem.Locals := ?lc;
+                       Opsem.Allocas := _
+                     |} :: _;
+       Opsem.Mem := _ |}  =>
+    let G := fresh "G" in
+    let gvs := fresh "gvs" in
+    assert (exists gvs, Opsem.getOperandValue td v lc gl = Some gvs) as G; 
+      try solve [
+        destruct H3 as [l5 [ps2 [cs21 H3]]]; subst;
+        destruct Hwfcfg1 as [_ [Hwfg1 [Hwfs1 HmInS1]]];
+        destruct Hwfpp1 as 
+          [_ [[Hreach1 [HbInF1 [HfInPs1 [_ [Hinscope1 _]]]]] _]];
+        inv_mbind;
+        eapply OpsemPP.getOperandValue_inTmnOperans_isnt_stuck; eauto 1;
+          simpl; auto
+      ];
+    destruct G as [gvs G]
+end.
+
+(* same to las *)
+Ltac tmnOps_eq H3 Hwfcfg1 Hwfpp1 HwfS1 :=
+      destruct H3 as [l1 [ps1 [cs11 H3]]]; subst;
+      destruct Hwfcfg1 as [_ [Hwfg1 [Hwfs1 HmInS1]]];
+      destruct Hwfpp1 as [_ [[Hreach1 [HbInF1 [HfInPs1 [_ [Hinscope1 _]]]]] _]];
+      destruct HwfS1 as [HwfS1 _];
+      unfold wf_ExecutionContext, inscope_of_ec in HwfS1;
+      inv_mbind;
+      eapply getOperandValue_inTmnOperands_sim; 
+        eauto 2 using wf_system__wf_fdef, wf_system__uniqFdef; simpl; auto.
+
+(* same to las *)
 Lemma s_isFinialState__laa_State_simulation: forall
   pinfo laainfo cfg1 FS1 cfg2 FS2
+  (Hwfcfg1: OpsemPP.wf_Config cfg1) (Hwfpp1: OpsemPP.wf_State cfg1 FS1) 
+  (Hwfcfg2: OpsemPP.wf_Config cfg2) (Hwfpp2: OpsemPP.wf_State cfg2 FS2) 
+  (HwfS1: id_rhs_val.wf_State (value_id (LAA_lid pinfo laainfo)) 
+           [! pinfo !] (PI_f pinfo) cfg1 FS1)
   (Hstsim : State_simulation pinfo laainfo cfg1 FS1 cfg2 FS2),
   Opsem.s_isFinialState cfg1 FS1 = Opsem.s_isFinialState cfg2 FS2.
-Admitted. (* sim *)
+Proof.
+  unfold Opsem.s_isFinialState.
+  intros.
+  destruct cfg2 as [S2 [los2 nts2] gl2 fs2].
+  destruct cfg1 as [S1 [los1 nts1] gl1 fs1].
+  destruct FS1 as [[|[? ? cs1 ? ?] ES1]]; 
+  destruct FS2 as [[|[? ? cs2 ? ?] ES2]]; try solve [
+    auto |
+    destruct Hstsim as [X [? [Hstsim [? [? ?]]]]]; subst; inv Hstsim
+  ].
+  destruct Hstsim as [X [? [Hstsim [? [? ?]]]]]; subst.
+  inv X. simpl.
+  destruct Hstsim as [Hstsim Hstsim'].
+  fold ECs_simulation in Hstsim'.
+  destruct Hstsim as [? [Htmn [? [? [? [? [? Hstsim]]]]]]]; subst.
+  destruct cs1, cs2; try solve [
+    auto |
+    apply cmds_simulation_nil_inv in Hstsim; try congruence |
+    apply cmds_simulation_nil_inv' in Hstsim; try congruence
+  ].
+  apply tmn_simulation__tmn_simulation' in Htmn.
+  inv Htmn; auto.
+    destruct ES1, ES2; try solve [auto | inv Hstsim'].
+      inTmnOp_isnt_stuck v H3 Hwfcfg1 Hwfpp1.
+      inTmnOp_isnt_stuck v' H4 Hwfcfg2 Hwfpp2.
+      rewrite G. rewrite G0.
+      f_equal.
+      tmnOps_eq H3 Hwfcfg1 Hwfpp1 HwfS1.
 
-Lemma undefined_state__laa_State_simulation_l2r: forall pinfo laainfo cfg1 St1 cfg2
-  St2 (Hstsim : State_simulation pinfo laainfo cfg1 St1 cfg2 St2),
-  OpsemPP.undefined_state cfg1 St1 -> OpsemPP.undefined_state cfg2 St2.
-Admitted. (* sim *)
+    destruct ES1, ES2; try solve [auto | inv Hstsim'].
+Qed.
 
-Lemma undefined_state__laa_State_simulation_r2l: forall pinfo laainfo cfg1 St1 cfg2
-  St2 (Hstsim : State_simulation pinfo laainfo cfg1 St1 cfg2 St2),
-  OpsemPP.undefined_state cfg2 St2 -> OpsemPP.undefined_state cfg1 St1.
-Admitted. (* sim *)
+(* same to las *)
+Ltac undefined_state__State_simulation_r2l_tac1 :=
+  match goal with
+  | Hstsim: State_simulation _ _ _ ?St1 _ ?St2 |- _ =>
+    destruct St2 as [[|[? ? [|CurCmds] [] ?] [|[]]] ?]; try tauto;
+    destruct CurCmds; try tauto;
+    destruct St1 as [ECS ?];
+    destruct Hstsim as [X [? [Hstsim [? [? ?]]]]]; subst;
+    inv X;
+    destruct ECS as [|[] ECS]; try tauto;
+    destruct Hstsim as [Hstsim Hstsim'];
+    destruct ECS as [|[] ECS]; try tauto;
+    destruct Hstsim as [? [Htmn [? [? [? [? [? Hstsim]]]]]]]; subst;
+    destruct Hstsim' as [Hstsim' _];
+    destruct Hstsim' as [? [? [? [? [? [? [? Hstsim']]]]]]]; subst;
+   simpl
+  end.
+
+(* same to las *)
+Ltac undefined_state__State_simulation_r2l_tac3 :=
+  match goal with
+  | Hstsim: State_simulation _ _ _ ?St1 _ ?St2 |- _ =>
+    destruct St2 as [[|[? [? ? ? tmn] CurCmds tmn' ?] ?] ?]; try tauto;
+    destruct tmn; try tauto;
+    destruct CurCmds; try tauto;
+    destruct tmn'; try tauto;
+    destruct St1 as [ECS ?];
+    destruct Hstsim as [X [? [Hstsim [? [? H3]]]]]; subst;
+    inv X;
+    destruct ECS as [|[] ECS]; try tauto;
+    destruct Hstsim as [Hstsim _];
+    destruct Hstsim as [? [Htmn [? [? [? [? [? Hstsim]]]]]]]; subst;
+    destruct H3 as [l5 [ps5 [cs5 EQ]]]; subst
+  end.
+
+(* same to las *)
+Ltac undefined_state__State_simulation_r2l_tac41 :=
+  match goal with
+  | Hstsim: State_simulation _ _ _ ?St1 ?cfg2 ?St2 |- _ =>
+    destruct St1 as [ECS ?];
+    destruct Hstsim as [X [? [Hstsim [? [? ?]]]]]; subst;
+    inv X;
+    destruct ECS as [|[? ? ? ? Locals0] ECS]; try tauto;
+    destruct Hstsim as [Hstsim _];
+    destruct Hstsim as [? [? [? [? [H4 [H5 [? Hstsim]]]]]]]; subst
+  end. 
+
+(* same to las *)
+Ltac undefined_state__la_State_simulation_r2l_tac42 := 
+repeat match goal with
+| Hwfcfg1: OpsemPP.wf_Config ?cfg1, Hwfpp1: OpsemPP.wf_State ?cfg1 ?St1, 
+  HwfS1: wf_State _ _ _ ?cfg1 ?St1, 
+  Hvsim: value_simulation _ _ _ ?v0 ?v,
+  _: ret ?gn = Opsem.getOperandValue ?td ?v ?Locals ?fs2,
+  _: block_simulation _ _ _ ?b _,
+  H4: exists _:_, exists _:_, exists _:_, ?b = _ |- _ =>
+    let G := fresh "G" in
+    let gvs := fresh "gvs" in
+    assert (exists gvs, Opsem.getOperandValue td
+       v0 Locals fs2 = Some gvs) as G; try solve [
+      destruct H4 as [l5 [ps2 [cs21 H4]]]; subst;
+      destruct Hwfcfg1 as [_ [Hwfg1 [Hwfs1 HmInS1]]];
+      destruct Hwfpp1 as [_ [[Hreach1 [HbInF1 [HfInPs1 [_ [Hinscope1 _]]]]] _]];
+      inv_mbind;
+      eapply OpsemPP.getOperandValue_inCmdOps_isnt_stuck; eauto 1; simpl; auto
+    ];
+    destruct G as [gvs G];
+    assert (gvs = gn) as EQ; try solve [
+      destruct H4 as [l1 [ps1 [cs11 H4]]]; subst;
+      destruct Hwfcfg1 as [_ [Hwfg1 [Hwfs1 HmInS1]]];
+      destruct Hwfpp1 as [_ [[Hreach1 [HbInF1 [HfInPs1 [_ [Hinscope1 _]]]]] _]];
+      destruct HwfS1 as [HwfS1 _];
+      unfold wf_ExecutionContext, inscope_of_ec in HwfS1;
+      inv_mbind;
+      eapply getOperandValue_inCmdOperands_sim; 
+        eauto 2 using wf_system__wf_fdef, wf_system__uniqFdef; simpl; auto
+    ];
+    subst;
+    clear Hvsim
+end.
+
+(* same to las *)
+Ltac undefined_state__la_State_simulation_r2l_tac43 := 
+      match goal with
+      | Hstsim: cmds_simulation _ _ _ _ (_::_) |- _ =>
+      apply cmds_simulation_cons_inv' in Hstsim; subst;
+      destruct Hstsim as [c1' [cs2' [J1 [J2 J3]]]]; subst;
+      apply cmd_simulation__cmd_simulation' in J2;
+      inv J2;
+      undefined_state__la_State_simulation_r2l_tac42
+     end.
+
+(* same to las *)
+Lemma undefined_state__laa_State_simulation_r2l: forall pinfo laainfo cfg1 St1 
+  cfg2 St2 (Hstsim : State_simulation pinfo laainfo cfg1 St1 cfg2 St2)
+  (Hwfcfg1: OpsemPP.wf_Config cfg1) (Hwfpp1: OpsemPP.wf_State cfg1 St1) 
+  (HwfS1: id_rhs_val.wf_State (value_id (LAA_lid pinfo laainfo)) 
+           [! pinfo !] (PI_f pinfo) cfg1 St1)
+  (Hundef: OpsemPP.undefined_state cfg2 St2), OpsemPP.undefined_state cfg1 St1.
+Proof.
+  intros.
+  unfold OpsemPP.undefined_state in Hundef.
+  destruct cfg2 as [S2 [los2 nts2] gl2 fs2].
+  destruct cfg1 as [S1 [los1 nts1] gl1 fs1].
+  repeat match goal with
+  | Hundef : _ \/ _ |- _ => destruct Hundef as [Hundef | Hundef]
+  end.
+  Case "1".
+
+    undefined_state__State_simulation_r2l_tac1.
+    apply cmds_simulation_nil_inv' in Hstsim; subst.
+    apply cmds_simulation_cons_inv' in Hstsim'.
+    destruct Hstsim' as [c1' [cs1' [J1 [J2 J3]]]]; subst.
+    left. 
+    unfold tmn_simulation in Htmn. 
+    destruct_if; subst; simpl; auto.
+    match goal with
+    | H11: subst_tmn _ _ ?tmn = insn_return _ _ _ |- _ => 
+      destruct tmn; inv H11; auto
+    end.
+
+  Case "2".
+    undefined_state__State_simulation_r2l_tac1.
+    apply cmds_simulation_nil_inv' in Hstsim; subst.
+    apply cmds_simulation_cons_inv' in Hstsim'.
+    destruct Hstsim' as [c1' [cs1' [J1 [J2 J3]]]]; subst.
+    right. left.
+    assert (getCallerReturnID c = getCallerReturnID c1') as EQ.
+      unfold cmd_simulation in J2. subst. clear.
+      destruct_if; auto.
+      destruct c1'; auto.
+    rewrite <- EQ.
+    clear - Htmn Hundef.
+    unfold tmn_simulation in Htmn. 
+    destruct (fdef_dec (PI_f pinfo) CurFunction1); subst; simpl; auto.
+    match goal with
+    | H11: subst_tmn _ _ ?tmn = insn_return_void _ |- _ => 
+      destruct tmn; inv H11; auto
+    end.
+
+  Case "3".
+
+    undefined_state__State_simulation_r2l_tac3.
+    apply cmds_simulation_nil_inv' in Hstsim. subst.
+    right. right. left.
+    simpl. 
+    unfold tmn_simulation in Htmn. 
+    destruct_if; subst; simpl; auto.
+    match goal with
+    | H11: subst_tmn _ _ ?tmn = insn_unreachable _ |- _ => 
+      destruct tmn; inv H11; auto
+    end.
+
+  Case "4".
+
+    right; right; right; left;
+    destruct St2 as [[|[? ? [|[] CurCmds] tmn' Locals] ?] ?]; try solve [
+      tauto |
+
+      inv_mbind; destruct Hundef as [gn [EQ Hundef]]; inv EQ; inv_mbind;
+      undefined_state__State_simulation_r2l_tac41;
+      undefined_state__la_State_simulation_r2l_tac43;
+        repeat fill_ctxhole; exists gn; fill_ctxhole; auto
+    ].
+
+  Case "5".
+    right. right. right. right. left.
+    destruct St2 as [[|[? ? [|[] CurCmds] tmn' ?] ?] ?]; try tauto.
+    inv_mbind; destruct Hundef as [gn [EQ Hundef]]; inv EQ; inv_mbind.
+    undefined_state__State_simulation_r2l_tac41.
+    undefined_state__la_State_simulation_r2l_tac43.
+    repeat fill_ctxhole; exists gn; fill_ctxhole; auto.
+
+  Case "6".
+    right. right. right. right. right. left.
+    destruct St2 as [[|[? ? [|[] CurCmds] tmn' ?] ?] ?]; try tauto.
+    inv_mbind; destruct Hundef as [gvs [EQ Hundef]]; inv EQ; inv_mbind.
+    undefined_state__State_simulation_r2l_tac41.
+    undefined_state__la_State_simulation_r2l_tac43. 
+    repeat fill_ctxhole; exists gvs; fill_ctxhole; auto.
+
+  Case "7".
+    right. right. right. right. right. right. left.
+    destruct St2 as [[|[? ? [|[] CurCmds] tmn' ?] ?] ?]; try tauto.
+    inv_mbind; destruct Hundef as [gv [mgv [EQ1 [EQ2 Hundef]]]]; 
+      inv EQ1; inv EQ2; inv_mbind.
+    undefined_state__State_simulation_r2l_tac41.
+    undefined_state__la_State_simulation_r2l_tac43. 
+    repeat fill_ctxhole; exists gv; exists mgv; fill_ctxhole; auto.
+
+  Case "8".
+    destruct St2 as [[|[? ? [|[] CurCmds] tmn' ?] ?] ?]; try tauto.
+    right; right; right; right. right. right. right.
+    undefined_state__State_simulation_r2l_tac41.
+    inv_mbind.
+    destruct Hundef as [fptr [EQ Hundef]]; inv EQ.
+    inv_mbind.
+    apply cmds_simulation_cons_inv' in Hstsim; subst;
+    destruct Hstsim as [c1' [cs2' [J1 [J2 J3]]]]; subst.
+    apply cmd_simulation__cmd_simulation' in J2;
+    inv J2.  
+    undefined_state__la_State_simulation_r2l_tac42.
+    repeat fill_ctxhole.
+    exists fptr. split; auto.
+    remember (OpsemAux.lookupExFdecViaPtr gl2 FunTable fptr) as R.
+    destruct R as [[[]]|].
+      inv_mbind.
+      destruct Hundef as [gvs0 [EQ Hundef]].
+      dgvs_instantiate_inv.
+      assert (exists gvs, 
+                Opsem.params2GVs (los2,nts2) lp0 Locals fs2 = Some gvs) as G'.
+        destruct H4 as [l5 [ps2 [cs21 H4]]]; subst.
+        destruct Hwfcfg1 as [_ [Hwfg1 [Hwfs1 HmInS1]]];
+        destruct Hwfpp1 as [_ [[Hreach1 [HbInF1 [HfInPs1 [_ [Hinscope1 _]]]]] _]].
+        inv_mbind.
+        eapply OpsemPP.params2GVs_isnt_stuck; eauto 1; simpl; auto.
+          exists nil. auto.
+      destruct G' as [gvs' G'].
+      assert (gvs' = l1) as EQ.
+        destruct H4 as [l5 [ps1 [cs11 H4]]]; subst;
+        destruct Hwfcfg1 as [_ [Hwfg1 [Hwfs1 HmInS1]]];
+        destruct Hwfpp1 as [_ [[Hreach1 [HbInF1 [HfInPs1 [_ [Hinscope1 _]]]]] _]];
+        destruct HwfS1 as [HwfS1 _];
+        unfold wf_ExecutionContext, inscope_of_ec in HwfS1;
+        inv_mbind.
+        eapply params2GVs_sim; 
+          eauto 2 using wf_system__wf_fdef, wf_system__uniqFdef; 
+            try solve [simpl; auto].
+      subst.
+      repeat fill_ctxhole.
+      erewrite TopSim.lookupFdefViaPtr__simulation_None_l2r; eauto.
+      erewrite TopSim.lookupExFdecViaPtr__simulation_r2l; eauto.
+      simpl.
+      exists l1. split; auto.
+    
+      erewrite TopSim.lookupFdefViaPtr__simulation_None_l2r; eauto.
+      erewrite TopSim.lookupExFdecViaPtr__simulation_None_r2l; eauto.
+Qed.
 
 Lemma sop_star__laa_State_simulation: forall pinfo laainfo cfg1 IS1 cfg2 IS2 tr
-  FS2 (Hwfpi: WF_PhiInfo pinfo) (Hwfcfg: OpsemPP.wf_Config cfg1) 
-  (Hwfpp: OpsemPP.wf_State cfg1 IS1) 
+  FS2 (Hwfpi: WF_PhiInfo pinfo) 
+  (Hwfcfg1: OpsemPP.wf_Config cfg1) (Hwfcfg2: OpsemPP.wf_Config cfg2) 
+  (Hwfpp1: OpsemPP.wf_State cfg1 IS1) (Hwfpp2: OpsemPP.wf_State cfg2 IS2) 
   (HwfS1: id_rhs_val.wf_State (value_id (LAA_lid pinfo laainfo)) 
            [! pinfo !] (PI_f pinfo) cfg1 IS1) alinfo Hp
   (Hsubst: substable_values (OpsemAux.CurTargetData cfg1) (OpsemAux.Globals cfg1)
@@ -1728,7 +2174,7 @@ Lemma sop_star__laa_State_simulation: forall pinfo laainfo cfg1 IS1 cfg2 IS2 tr
   (Hless: 0 <= maxb) (Hwfgs: MemProps.wf_globals maxb (OpsemAux.Globals cfg1))
   (Hnoalias: Promotability.wf_State maxb pinfo cfg1 IS1)
   (Hstsim : State_simulation pinfo laainfo cfg1 IS1 cfg2 IS2)
-  (Hopstar : Opsem.sop_star cfg2 IS2 FS2 tr),
+  (Hopstar : Opsem.sop_star cfg2 IS2 FS2 tr) (Hok: ~ sop_goeswrong cfg1 IS1),
   exists FS1, Opsem.sop_star cfg1 IS1 FS1 tr /\
     State_simulation pinfo laainfo cfg1 FS1 cfg2 FS2.
 Proof.
@@ -1738,13 +2184,17 @@ Proof.
   induction Hopstar; intros.
     exists IS1. split; auto.
 
-    assert (J:=Hwfpp).
-    apply OpsemPP.progress in J; auto.
-    destruct J as [Hfinal1 | [[IS1' [tr0 Hop1]] | Hundef1]].
-      apply s_isFinialState__laa_State_simulation in Hstsim.
+    assert (forall (Hfinal1: Opsem.s_isFinialState cfg1 IS1 <> merror),
+            exists FS1 : Opsem.State,
+              Opsem.sop_star cfg1 IS1 FS1 (tr1 ** tr2) /\
+              State_simulation pinfo laainfo cfg1 FS1 cfg2 state3) as W.
+      intros.
+      apply s_isFinialState__laa_State_simulation in Hstsim; auto.
       rewrite Hstsim in Hfinal1.
       contradict H; eauto using s_isFinialState__stuck.
-
+    assert (J:=Hwfpp1).
+    apply OpsemPP.progress in J; auto.
+    destruct J as [Hfinal1 | [[IS1' [tr0 Hop1]] | Hundef1]]; auto.
       eapply laa_is_sim in Hstsim; eauto.
       destruct Hstsim as [Hstsim EQ]; subst.
       assert (OpsemPP.wf_State cfg1 IS1') as Hwfpp'.
@@ -1759,13 +2209,17 @@ Proof.
         eapply alive_alloca.preservation in Hop1; eauto.
       assert (Promotability.wf_State maxb pinfo cfg1 IS1') as Hnoalias'.
         eapply Promotability.preservation in Hop1; eauto.
-      eapply IHHopstar in Hstsim; eauto.
+      eapply IHHopstar in Hstsim; 
+        eauto using sop_goeswrong__step, (@OpsemPP.preservation DGVs).
       destruct Hstsim as [FS1 [Hopstar1 Hstsim]].
       exists FS1.
       split; eauto.
 
-      eapply undefined_state__laa_State_simulation_l2r in Hstsim; eauto.
-      contradict H; eauto using undefined_state__stuck.
+      apply undefined_state__stuck' in Hundef1.
+      remember (Opsem.s_isFinialState cfg1 IS1) as R.
+      destruct R.
+        apply W; congruence.
+        contradict Hok. exists IS1. exists E0. split; auto.
 Qed.
 
 Lemma sop_div__laa_State_simulation: forall pinfo laainfo cfg1 IS1 cfg2 IS2 tr
@@ -1826,6 +2280,47 @@ Lemma laa_wfS: forall (los : layouts) (nts : namedts) (fh : fheader)
 Proof.
 Admitted. (* WF prev *)
 
+Lemma vev_State_preservation : forall pinfo laainfo cfg IS maxb
+  (Hwfg: MemProps.wf_globals maxb (OpsemAux.Globals cfg))
+  (Halias: Promotability.wf_State maxb pinfo cfg IS) (Hwfpi: WF_PhiInfo pinfo)
+  alinfo Hp (Hlas2st : exist _ alinfo Hp = laainfo__alinfo pinfo laainfo)
+  (Halst: alive_alloca.wf_State pinfo alinfo cfg IS)
+  (Hwfcfg : OpsemPP.wf_Config cfg) (Hwfpp: OpsemPP.wf_State cfg IS) 
+  (Hvev: vev_State (value_id (LAA_lid pinfo laainfo))
+               [! pinfo !] (PI_f pinfo) cfg IS)
+  IS' tr  (Hstep: Opsem.sInsn cfg IS IS' tr),
+  vev_State (value_id (LAA_lid pinfo laainfo))
+               [! pinfo !] (PI_f pinfo) cfg IS'.
+Proof.
+  intros.
+  eapply laa__alive_alloca__vev; eauto.
+    apply OpsemPP.preservation in Hstep; auto.
+    eapply alive_alloca.preservation in Hstep; eauto.
+Qed.
+
+Lemma id_rhs_val_preservation_star : forall v1 v2 F pinfo laainfo cfg IS IS' tr
+  (Heq1: v1 = value_id (LAA_lid pinfo laainfo))
+  (Heq2: v2 = [! pinfo !]) (Heq3: F = PI_f pinfo) maxb (Hle: 0 <= maxb)
+  (Hwfg: MemProps.wf_globals maxb (OpsemAux.Globals cfg))
+  (Halias: Promotability.wf_State maxb pinfo cfg IS) (Hwfpi: WF_PhiInfo pinfo)
+  alinfo Hp (Hlas2st : exist _ alinfo Hp = laainfo__alinfo pinfo laainfo)
+  (Halst: alive_alloca.wf_State pinfo alinfo cfg IS)
+  (Hvals : substable_values (OpsemAux.CurTargetData cfg) (OpsemAux.Globals cfg)
+             F v1 v2) (Hvev: vev_State v1 v2 F cfg IS) 
+  (Hwfcfg : OpsemPP.wf_Config cfg) (Hwfpp: OpsemPP.wf_State cfg IS) 
+  (HwfS1: id_rhs_val.wf_State v1 v2 F cfg IS) (Hstar: Opsem.sop_star cfg IS IS' tr),
+  id_rhs_val.wf_State v1 v2 F cfg IS'.
+Proof.
+  intros. subst.
+  induction Hstar; auto.
+    apply IHHstar; auto.
+      eapply Promotability.preservation; eauto.
+      eapply alive_alloca.preservation; eauto.
+      eapply OpsemPP.preservation; eauto.
+      eapply vev_State_preservation; eauto.
+      eapply id_rhs_val.preservation; eauto.
+Qed.  
+
 Lemma laa_sim: forall (los : layouts) (nts : namedts) (fh : fheader)
   (dones : list id) (pinfo : PhiInfo) (main : id) (VarArgs : list (GVsT DGVs))
   (bs1 : list block) (l0 : l) (ps0 : phinodes) (cs0 : cmds) (tmn0 : terminator)
@@ -1872,19 +2367,18 @@ Proof.
     constructor; auto.
     repeat split; auto.
     simpl in Huniq. destruct Huniq as [[_ [_ Huniq]] _].
-    unfold TopSim.products_simulation. unfold fsim. unfold Fsim.
+    unfold TopSim.products_simulation. unfold fsim. unfold Fsim. 
     apply uniq_products_simulation; auto.
   assert (uniqFdef (PI_f pinfo)) as HuniqF.
     admit. (* wfF *)
-  constructor; auto.
-    intros tr t Hconv.
-    inv Hconv.
 
 Ltac laa_sim_init :=
 match goal with
-| H: Opsem.s_genInitState [module_intro ?los ?nts _] _ _ _ = _,  
+| H: Opsem.s_genInitState [module_intro ?los ?nts _] _ _ _ = Some (?cfg, ?IS),  
   pinfo: PhiInfo, laainfo: LAAInfo _
   |- _ =>
+    assert (OpsemPP.wf_Config cfg /\ OpsemPP.wf_State cfg IS) as Hwfst';
+      try solve [eapply s_genInitState__opsem_wf in H; eauto using laa_wfS];
     eapply s_genInitState__laa_State_simulation in H; eauto;
     destruct H as [cfg1 [IS1 [Hinit Hstsim]]];
     assert (OpsemPP.wf_Config cfg1 /\ OpsemPP.wf_State cfg1 IS1) as Hwfst;
@@ -1912,12 +2406,36 @@ match goal with
       try solve [eapply s_genInitState__alive_alloca; eauto]
 end.
 
+Ltac laa_sim_end :=
+ match goal with
+| Hstsim' : State_simulation ?pinfo ?laainfo ?cfg1 ?FS1 ?cfg ?FS,
+  Hopstar1 : Opsem.sop_star ?cfg1 _ ?FS1 _ |- _ =>
+    assert (OpsemPP.wf_State cfg FS) as Hwfst''; 
+      try solve [eapply OpsemPP.preservation_star; eauto; try tauto];
+    assert (OpsemPP.wf_State cfg1 FS1) as Hwfst1'';
+      try solve [eapply OpsemPP.preservation_star; eauto; try tauto];
+    assert (wf_State (value_id (LAA_lid pinfo laainfo)) [! pinfo !]
+      (PI_f pinfo) cfg1 FS1); try solve [
+      eapply id_rhs_val_preservation_star in Hopstar1; eauto; try solve [
+        tauto |
+        eapply laa__alive_alloca__vev; eauto; try tauto
+      ]
+    ]
+end.
+
+  constructor; auto.
+    intros tr t Hconv.
+    inv Hconv.
     laa_sim_init.
-    eapply sop_star__laa_State_simulation in Hstsim; eauto; try tauto.
+    eapply sop_star__laa_State_simulation in Hstsim; 
+      eauto using defined_program__doesnt__go_wrong; try tauto.
     destruct Hstsim as [FS1 [Hopstar1 Hstsim']].
+    laa_sim_end.
     match goal with
-    | H1: Opsem.s_isFinialState _ _ = _ |- _ =>
-      erewrite <- s_isFinialState__laa_State_simulation in H1; eauto
+    | Hstsim' : State_simulation _ _ _ _ ?cfg ?FS,
+      H: Opsem.s_isFinialState ?cfg ?FS = _ |- _ =>
+      eapply s_isFinialState__laa_State_simulation in Hstsim'; eauto; try tauto;
+      rewrite <- Hstsim' in H
     end.
     econstructor; eauto.
 
@@ -1937,9 +2455,12 @@ end.
     assert (OpsemPP.undefined_state cfg t) as Hundef.
       apply stuck__undefined_state in H2; try solve [auto | tauto].
     laa_sim_init.
-    eapply sop_star__laa_State_simulation in Hstsim; eauto; try tauto.
+    eapply sop_star__laa_State_simulation in Hstsim;
+      eauto using defined_program__doesnt__go_wrong; try tauto.
     destruct Hstsim as [FS1 [Hopstar1 Hstsim']].
-    eapply Promotability.preservation_star in Hprom; eauto; try tauto.
+    assert (Hprom':=Hprom).
+    eapply Promotability.preservation_star in Hprom'; eauto; try tauto.
+    laa_sim_end.
     assert (OpsemPP.undefined_state cfg1 FS1) as Hundef'.
       eapply undefined_state__laa_State_simulation_r2l in Hundef; 
         try solve [eauto | tauto].
