src3.0/Transforms/trans_tactic.v
@@ -119,3 +119,5 @@ repeat match goal with
        rewrite_env (A++[a]++nil) in H;
        contradict H; simpl; apply app_cons_not_nil
 end.
+
+
